dimsum_examples/compiler/codegen.v
@@ -19,7 +19,7 @@ Inductive error :=
 | AssertionFailed (s : string)
 | TooManyArgs
 .
-
+ 
 Definition variable_registers : list string :=
   ["R19"; "R20"; "R21"; "R22"; "R23"; "R24"; "R25"; "R26"; "R27"; "R28"; "R29"].
 
